revert to lean, added decidability instances

MyProject/gossip.lean
@@ -1,6 +1,6 @@
 import Mathlib.Data.List.Basic
 import Mathlib.Data.Fin.Basic
-
+import Mathlib.Data.Fintype.Basic
 
 variable {n : ℕ}
 
@@ -10,30 +10,73 @@ def Call (n : Nat): Type := Fin n × Fin n
 
 def generateState (n : Nat) : GossipState n := fun i j => i = j
 
+instance {n : ℕ} : DecidableRel (generateState n) := decEq
+
+-- Determines if someone is an expert
+-- a is agent, n is the total number of secrets
+def isExpert (s : GossipState n) (i : Fin n): Prop := ∀ j, s i j
+
+instance {s : GossipState n} [DecidableRel s] {i : Fin n} : Decidable (isExpert s i) :=
+  Fintype.decidableForallFintype
+
+-- Checks if everyone is an expert
+def checkIfEE (s : GossipState n) : Prop := ∀ i, isExpert s i
+
+instance {s : GossipState n} [DecidableRel s] : Decidable (checkIfEE s) :=
+  Fintype.decidableForallFintype
+
 def makeCall (s : GossipState n) : Call n → GossipState n
-| (i, j), x, y =>
+  | (i, j), x, y =>
     if x = i
-      then s x y ∨ s j y
+    then s x y ∨ s j y
+    else
+      if x = j
+        then s x y ∨ s i y
+        else s x y
+
+instance {s : GossipState n} [DecidableRel s] : ∀ {c : Call n}, DecidableRel (makeCall s c)
+| (i, j), x, y =>
+    if h : x = i
+      then decidable_of_iff (s i y ∨ s j y) (by simp [makeCall, h])
       else
-        if x = j
-          then s x y ∨ s i y
-          else s x y
+        if h' : x = j
+          then decidable_of_iff (s j y ∨ s i y) (by cases h'; simp [makeCall, h])
+          else decidable_of_iff (s x y) (by simp [makeCall, h, h'])
+
 
 def makeCalls (s : GossipState n) (cs : List (Call n)) : GossipState n :=
   cs.foldl makeCall s
 
+instance {s : GossipState n} [DecidableRel s] {cs : List (Call n)} :
+    DecidableRel (makeCalls s cs) := by
+  induction cs generalizing s
+  case nil hs => exact hs
+  case cons c _ ih hs => exact ih
+
 def everyoneExpert (s : GossipState n) : Prop := ∀ a b : Fin n, s a b
 
 -- Prop: are two states identical?
-def moreGossip (s1 s2 : GossipState n) : Prop := ∀ a b : Fin n, s1 a b → s2 a b
+def moreGossip (s1 s2 : GossipState n) : Prop := ∀ a b : Fin n, (s1 a b) → (s2 a b)
+
+-- Adds an agent to a state, that knows only their own secret
+def addAgent (s : GossipState n) : GossipState (n.succ) :=
+  λ a b => by
+  cases a using Fin.lastCases
+  case last => -- if a = n.succ (the new agent)
+    exact b == n.succ
+  case cast i =>
+    cases b using Fin.lastCases
+    · exact false -- old agent a should not know secrets of the new agent
+    case cast b =>
+      exact s i b -- old agent a should know secrets of another old agent b iff that was already the case before.
 
 -- Doing a call and some list after is the same as doing a list of calls with that call as its head
 lemma makeCalls_cons (s : GossipState n) (c : Call n) (cs : List (Call n)) :
-    makeCalls s (c :: cs) = makeCalls (makeCall s c) cs := by
+  makeCalls s (c :: cs) = makeCalls (makeCall s c) cs := by
     rfl
 
-lemma makeCall_increases_gossip (s1 s2 : GossipState n) (c : Call n) :
-    moreGossip s1 s2 → moreGossip (makeCall s1 c) (makeCall s2 c) := by
+lemma makeCall_increases_gossip (s1 s2 : GossipState n) (c : Call
+n) : moreGossip s1 s2 → moreGossip (makeCall s1 c) (makeCall s2 c) := by
     intro h
     intro a b
     simp [makeCall]
@@ -52,20 +95,8 @@ lemma makeCall_increases_gossip (s1 s2 : GossipState n) (c : Call n) :
     aesop_subst
       h_1
     simp_all only [↓reduceIte]
-    unhygienic
-      aesop_cases
-        a_1
-    · apply
-        Or.inl
-      apply
-        h
-      simp_all only
-    · apply
-        Or.inr
-      apply
-        h
-      simp_all only
-    aesop
+    aesop?
+    aesop?
 
 -- doing a call doesnt decrease the amount of gossip
 lemma makeCall_makes_gossip (s : GossipState n) (c : Call n) :
@@ -105,11 +136,13 @@ lemma makeCalls_increases_gossip (s1 s2 : GossipState n) (cs : List (Call n)) :
       exact h
     case cons head tail ih =>
       rw [makeCalls_cons, makeCalls_cons]
-      have h_call : moreGossip (makeCall s1 head) (makeCall s2 head) := makeCall_increases_gossip s1 s2 head h
+      have h_call : moreGossip (makeCall s1 head) (makeCall s2
+      head) := makeCall_increases_gossip s1 s2 head h
       exact ih (makeCall s1 head) (makeCall s2 head) h_call
 
 -- Before some arbitrary call, the same information is still available.
-lemma knowledge_persists_call_before (n : ℕ) (σ : List (Call n)) (i j k l: Fin n) :
+lemma knowledge_persists_call_before (n : ℕ) (σ : List (Call n))
+(i j k l: Fin n) :
   (makeCalls (generateState n) σ i j) →
   (makeCalls (makeCall (generateState n) (k, l)) σ) i j := by
   intro h
@@ -119,32 +152,52 @@ lemma knowledge_persists_call_before (n : ℕ) (σ : List (Call n)) (i j k l: Fi
 
 
 lemma knowledge_persists_call_after (n : ℕ) (σ : List (Call n)) (i j k l: Fin n) :
-  (makeCalls (generateState n) σ i j) →
-  (makeCall (makeCalls (generateState n) σ) (k, l)) i j := by
+  (makeCalls (generateState n) σ i j) → (makeCall (makeCalls (generateState n) σ) (k, l)) i j := by
   simp [makeCall]
   intro h
   if h_eq : i = k then
-    rw [h_eq]
-    rw [if_pos]
+    rw [if_pos h_eq]
     left
-    rw [← h_eq]
-    case h =>
-      exact h
-    case hc =>
-      rfl
+    exact h
   else
     rw [if_neg h_eq]
     if h_eq2 : i = l then
-      rw [h_eq2]
-      rw [if_pos]
+      rw [if_pos h_eq2]
       left
-      rw [← h_eq2]
       exact h
-      case hc => -- WHY IS THIS NECESSARY????
-        rfl
     else
       rw [if_neg h_eq2]
       exact h
 
+lemma inductive_case : ∀ (k : Nat), (Nat.succ k + 4 ≥ 4) → (∃ seq, checkIfEE (makeCalls (generateState (k + 4)) seq))
+  → ∃ seq', checkIfEE (makeCalls (generateState (Nat.succ k + 4)) seq') := by
+  intro n h IH
+  cases IH
+  rename_i k seq IH
+  let zero_fin : Fin (k + 5) := Fin.ofNat 0
+  let succ_fin : Fin (k + 5) := Fin.ofNat (Nat.succ n)
+  let initial_call : List (Call (k + 5))  := [(zero_fin, succ_fin)]
+  sorry
 
--- Next goal, set up the final goal with sorry's and start proving the lemmas.
+  -- We know that there is a sequence of calls that makes everyone an expert
+  -- First step is to add a new agent
+  -- We know that the new agent knows only their own secret
+  -- We know that the old agents know all (old) secrets when call sequence sigma is applied
+  -- after adding a new call from agent 0 to the new agent at the start,
+
+-- induction for n > 3, base case n = 4
+theorem expertSequenceWorks (n : Nat) : (n ≥ 4) → ∃ (seq : List (Call n)), checkIfEE (makeCalls (generateState n) seq) :=
+  match n with
+  | 0 => by simp
+  | 1 => by simp
+  | 2 => by simp
+  | 3 => by simp
+  | (m + 4) =>  by
+                intro h
+                induction m
+                case zero =>
+                  simp at h
+                  exists [(0, 1), (2, 3), (0, 2), (1, 3)]
+                case succ k IH =>
+                  simp at IH
+                  exact inductive_case k h IH
